Fixing and extending theories affected by the addition of IsNullNode and FixedGuardNode

Graph/Values.thy
@@ -263,7 +263,8 @@ fun intval_conditional :: "Value \<Rightarrow> Value \<Rightarrow> Value \<Right
   "intval_conditional cond tv fv = (if (val_to_bool cond) then tv else fv)"
 
 fun intval_is_null :: "Value \<Rightarrow> Value" where
-  "intval_is_null v = (if (v = ObjRef (None)) then bool_to_val True else bool_to_val False)"
+  "intval_is_null (ObjRef (v)) = (if (v=(None)) then bool_to_val True else bool_to_val False)" |
+  "intval_is_null _ = UndefVal"
 
 subsection \<open>Narrowing and Widening Operators\<close>
 
